## Implicitly Defined Functions

So far, we have worked mostly with **explicit functions**, where one variable is written directly in terms of another, for example:
- $y = x^3 + 1$
- $y = x \sin x$

In these cases, $y$ is expressed *explicitly* as a function of $x$.  
However, sometimes the relationship between $x$ and $y$ is given **implicitly**, by an equation like:
- $x^2 + y^2 = 25$
- $x^3 + y^3 = 6xy$

These equations relate $x$ and $y$ without solving for $y$.  
For instance, $x^2 + y^2 = 25$ defines a **circle** of radius 5 centered at the origin.

If we solve for $y$, we get:
$$y = \pm \sqrt{25 - x^2}$$
The “$+$” gives the upper semicircle, and the “$−$” gives the lower semicircle.  
Both are *implicitly defined* by the same equation.

But for more complex relations (like $x^3 + y^3 = 6xy$), solving for $y$ explicitly is **difficult or impossible**.  
Instead, we use a technique called **implicit differentiation**.
![[Pasted image 20251028145509.png]]
---

## Implicit Differentiation — The Idea

We can find $\dfrac{dy}{dx}$ **without** explicitly solving for $y$.

**Method:**
1. Differentiate both sides of the equation with respect to $x$.
2. Remember that $y$ depends on $x$ → use the **Chain Rule** when differentiating any term with $y$.
3. Solve the resulting equation for $\dfrac{dy}{dx}$.

> [!note] (Key Concept)
> When differentiating implicitly, treat $y$ as a function of $x$ and apply:
> $$\frac{d}{dx}(y^n) = n y^{n-1} \frac{dy}{dx}$$
![[Pasted image 20251028145535.png]]

---

## Example 1: Circle $x^2 + y^2 = 25$

### Step 1: Differentiate both sides
$$\frac{d}{dx}(x^2 + y^2) = \frac{d}{dx}(25)$$
$$2x + 2y \frac{dy}{dx} = 0$$

### Step 2: Solve for $\dfrac{dy}{dx}$
$$\frac{dy}{dx} = -\frac{x}{y}$$

So, the slope of the tangent line at any point $(x, y)$ on the circle is $-\frac{x}{y}$.

---

### Example: Tangent at (3, 4)
At $(3, 4)$:
$$\frac{dy}{dx} = -\frac{3}{4}$$

Equation of the tangent line:
$$y - 4 = -\frac{3}{4}(x - 3)$$
or equivalently:
$$3x + 4y = 25$$

> [!note] (Observation)
> Even if we can solve for $y = \sqrt{25 - x^2}$, implicit differentiation is **simpler** and avoids extra algebraic work.
![[Pasted image 20251028145602.png]]

---

## Example 2: The Folium of Descartes

Equation:
$$x^3 + y^3 = 6xy$$

### (a) Find $y'$.

Differentiate both sides w.r.t. $x$:
$$3x^2 + 3y^2 y' = 6y + 6x y'$$

Group the $y'$ terms:
$$3y^2 y' - 6x y' = 6y - 3x^2$$

Factor out $y'$:
$$y'(3y^2 - 6x) = 6y - 3x^2$$

Solve for $y'$:
$$y' = \frac{6y - 3x^2}{3y^2 - 6x} = \frac{2y - x^2}{y^2 - 2x}$$
![[Pasted image 20251028145653.png]]
---

### (b) Tangent at $(3, 3)$

Substitute $x = 3$, $y = 3$:
$$y' = \frac{2(3) - 9}{9 - 6} = \frac{6 - 9}{3} = -1$$

Equation of tangent:
$$y - 3 = -1(x - 3) \Rightarrow x + y = 6$$

---

### (c) When is the tangent horizontal?

A tangent is **horizontal** when $y' = 0$:
$$2y - x^2 = 0 \Rightarrow y = \frac{x^2}{2}$$

Substitute into the original equation:
$$x^3 + \left(\frac{x^2}{2}\right)^3 = 6x\left(\frac{x^2}{2}\right)$$
Simplify:
$$x^3 + \frac{x^6}{8} = 3x^3 \Rightarrow x^6 - 16x^3 = 0$$
$$x^3 = 16 \Rightarrow x = \sqrt[3]{16} \approx 2.52$$

Then:
$$y = \frac{x^2}{2} \approx 3.17$$

So, the tangent is horizontal at approximately $(2.52, 3.17)$.

---

## Example 3: $\sin(x + y) = y^2 \cos x$

Differentiate both sides w.r.t. $x$:
$$\cos(x + y)(1 + y') = 2y y' \cos x - y^2 \sin x$$

Now collect $y'$ terms:
$$\cos(x + y) + \cos(x + y)y' = 2y y' \cos x - y^2 \sin x$$

Bring all $y'$ terms to one side:
$$\cos(x + y)y' - 2y y' \cos x = -\cos(x + y) - y^2 \sin x$$

Factor out $y'$:
$$y'[\cos(x + y) - 2y \cos x] = -[\cos(x + y) + y^2 \sin x]$$

Solve for $y'$:
$$y' = \frac{-\cos(x + y) - y^2 \sin x}{\cos(x + y) - 2y \cos x}$$

> Check: at $(0, 0)$, $y' = -1$.  
> The graph’s slope near the origin confirms this result.

---

## Second Derivatives of Implicit Functions

To find $y''$, first find $y'$, then **differentiate again**, remembering that $y$ is still a function of $x$.

### Example 4: $x^4 + y^4 = 16$

Differentiate once:
$$4x^3 + 4y^3 y' = 0 \Rightarrow y' = -\frac{x^3}{y^3}$$

Differentiate again using the **Quotient Rule**:
$$y'' = \frac{d}{dx}\left(-\frac{x^3}{y^3}\right)$$

Compute derivative:
$$y'' = \frac{-3x^2 y^3 - (-x^3)(3y^2 y')}{y^6}$$

Simplify:
$$y'' = \frac{-3x^2 y^3 + 3x^3 y^2 y'}{y^6} = \frac{3x^2(-y + x y')}{y^4}$$

Substitute $y' = -\dfrac{x^3}{y^3}$:
$$y'' = \frac{3x^2(-y + x(-\frac{x^3}{y^3}))}{y^4} = \frac{-3x^2(y^4 + x^4)}{y^7}$$

From the original equation $x^4 + y^4 = 16$:
$$y'' = \frac{-3x^2(16)}{y^7} = -\frac{48x^2}{y^7}$$

---

## Summary of Implicit Differentiation Steps

1. Differentiate both sides w.r.t. $x$.  
2. Use the **Chain Rule** for $y$ terms.  
3. Collect all terms with $\dfrac{dy}{dx}$.  
4. Factor and solve for $\dfrac{dy}{dx}$.  
5. (Optional) Substitute $y'$ back to find higher derivatives.

> [!note] (Why Use Implicit Differentiation?)
> - It avoids the need to solve complex equations for $y$.  
> - Works for curves that define multiple branches (like circles or foliums).  
> - Extends naturally to higher derivatives.