## 2.2 The Idea of Elimination (detailed vázlat)

### Basic concept
- **Goal**: systematically solve linear systems by removing variables step by step  
- **Unknowns**: $x_1, x_2, x_3$ (for $n=3$)  
- **Equations**:  
$$
\begin{cases}
\text{eq1}: a_{11}x_1 + a_{12}x_2 + a_{13}x_3 = b_1 \\
\text{eq2}: a_{21}x_1 + a_{22}x_2 + a_{23}x_3 = b_2 \\
\text{eq3}: a_{31}x_1 + a_{32}x_2 + a_{33}x_3 = b_3
\end{cases}
$$  
- **Magyarul**: az ismeretlenek fokozatos kiküszöbölése a cél  

---

### Step 1: Eliminate the first variable
1. Pick **pivot**: first nonzero coefficient in eq1, $a_{11}$  
2. Compute **multiplier** for eq2: $m = a_{21}/a_{11}$  
3. Subtract $m \cdot$ eq1 from eq2 → $x_1$ eliminated from eq2  
4. Repeat for all remaining equations to eliminate $x_1$  
- **Magyarul**: az első ismeretlen eltüntetése sorok lineáris kombinációjával  

#### Example 2x2
- System:  
$$
\begin{cases}
x - 2y = 1 \\
3x + 2y = 11
\end{cases}
$$  
- Multiply eq1 by 3: $3x - 6y = 3$  
- Subtract from eq2: $(3x + 2y) - (3x - 6y) = 8y$ → $8y = 8$  
- Solve for $y$: $y = 1$  
- Back substitute to find $x$: $x - 2\cdot1 = 1 \Rightarrow x = 3$  
- **Magyarul**: eltüntetés után visszahelyettesítéssel oldunk  
![[Pasted image 20251001190356.png]]
---

### Step 2: Triangular system
- After elimination, the system becomes **upper triangular**:  
$$
\begin{cases}
x_1 + ... = ... \\
0 + x_2 + ... = ... \\
0 + 0 + x_3 = ...
\end{cases}
$$  
- **Back substitution**: solve bottom-to-top  
- **Magyarul**: háromszög rendszer → alulról felfelé oldunk  

---

### Pivot and multiplier
- **Pivot**: first nonzero entry in the row performing elimination ($a_{11}$)  
- **Multiplier**: entry to eliminate / pivot ($a_{21}/a_{11}$)  
- Example:  
  - Change eq1 to $4x - 8y = 4$  
  - To eliminate $3x$ in eq2: $m = 3/4$  
  - Subtract $3/4 \cdot$ eq1 from eq2 → new eq2: $8y = 8$ → $y=1$  
- **Magyarul**: pivot → vezető együttható, multiplier → szorzó a kiküszöböléshez  

---

### Step 3: Repeat for other variables
- After eliminating $x_1$, use new pivot ($x_2$ coefficient) to eliminate $x_2$ from remaining equations  
- Continue until all $n$ unknowns are eliminated except in one equation  
- Solve by **back substitution**  

---

### Important notes
1. Elimination may **break down** if a pivot = 0 → may require **row exchanges**  
2. Multipliers and pivots define the **triangular structure** of the system  
3. The original solution remains unchanged throughout elimination  
- **Magyarul**: a módszer stabil, de pivot = 0 esetén sorcsere szükséges; a megoldás mindig ugyanaz marad  

---

### Summary
- **Elimination** = systematic removal of variables  
- Produces **upper triangular system**  
- Solve using **back substitution**  
- Pivots and multipliers are key concepts for elimination  
- **Magyarul**: a kiküszöbölés logikus sorrendben törli a változókat, a háromszög rendszerből visszahelyettesítéssel oldunk  

### Pivot and Multiplier (detailed explanation and examples)

- **Pivot**: the first nonzero coefficient in the current row used to eliminate the corresponding variable in other rows.  
  - It is the “reference” number for the elimination step.  
  - Example: consider the system  
    $$
    \begin{cases}
    x - 2y = 1 \\
    3x + 2y = 11
    \end{cases}
    $$  
    - First pivot: $a_{11} = 1$ (coefficient of $x$ in the first row)  

- **Multiplier**: the factor used to eliminate the variable in another row, calculated as  
$$
\text{multiplier} = \frac{\text{entry to eliminate}}{\text{pivot}}
$$  
  - In the example: to eliminate $x$ from the second equation: $m = a_{21}/a_{11} = 3/1 = 3$  
  - Perform elimination:  
$$
(3x + 2y) - 3(x - 2y) = 3x + 2y - 3x + 6y = 8y
$$  
  - The $x$ term is eliminated. The second equation now gives $8y = 8 \Rightarrow y = 1$  
  - **Explanation**: multiplying the first equation by the multiplier ensures that the $x$ terms in the second row cancel exactly.  

#### Changing the pivot
- Suppose the first equation is changed to $4x - 8y = 4$ (same line, different scaling)  
  - New pivot: $a_{11} = 4$  
  - Multiplier for second row: $m = a_{21}/a_{11} = 3/4$  
  - Subtract:  
$$
3x + 2y - \frac{3}{4}(4x - 8y) = 3x + 2y - (3x - 6y) = 8y
$$  
  - Solve: $y = 1$  
  - Back substitution: $4x - 8 = 4 \Rightarrow 4x = 12 \Rightarrow x = 3$  
  - **Explanation**: changing the pivot scales the elimination step, but the solution remains unchanged.  

---

### Eliminating variables in larger systems
- Step 1: select the first pivot (top-left entry)  
- Step 2: compute multipliers for all rows below to eliminate that variable  
- Step 3: subtract multiples of the pivot row from the rows below  
- Step 4: move to the next pivot (second row, second column after elimination)  
- Repeat until all variables except one in the last equation are eliminated  

#### Example: 3×3 system
System:  
$$
\begin{cases}
x + 2y + 3z = 6 \\
2x + 5y + 2z = 4 \\
6x - 3y + z = 2
\end{cases}
$$

**Step 1: eliminate $x$ from eq2 and eq3**  
- Pivot: $a_{11} = 1$  
- Multiplier for eq2: $m_{21} = 2/1 = 2$  
- Multiply eq1 by 2 and subtract from eq2:  
$$
(2x + 5y + 2z) - 2(x + 2y + 3z) = (2x - 2x) + (5y - 4y) + (2z - 6z) = y - 4z
$$  
- New eq2: $y - 4z = 4 - 12 = -8$  

- Multiplier for eq3: $m_{31} = 6/1 = 6$  
- Multiply eq1 by 6 and subtract from eq3:  
$$
(6x - 3y + z) - 6(x + 2y + 3z) = -15y - 17z
$$  
- New eq3: $-15y - 17z = 2 - 36 = -34$  

**Step 2: eliminate $y$ from eq3**  
- Pivot: new eq2 first coefficient of $y = 1$  
- Multiplier for eq3: $m_{32} = -15/1 = -15$  
- Subtract $-15 \cdot$ eq2 from eq3:  
$$
(-15y - 17z) - (-15)(y - 4z) = (-15y - 17z) + 15y - 60z = -77z
$$  
- New eq3: $-77z = -34 - (-15 \cdot -8) = -34 - 120 = -154$  

**Step 3: back substitution**  
- Solve last equation for $z$: $-77z = -154 \Rightarrow z = 2$  
- Substitute $z=2$ into eq2: $y - 4\cdot2 = -8 \Rightarrow y - 8 = -8 \Rightarrow y=0$  
- Substitute $y=0, z=2$ into eq1: $x + 2\cdot0 + 3\cdot2 = 6 \Rightarrow x + 6 = 6 \Rightarrow x=0$  

**Step 4: final solution**  
$$
(x, y, z) = (0, 0, 2)
$$  

- **Explanation**:  
  - Each pivot defines the variable to eliminate in rows below  
  - Multipliers ensure exact cancellation of that variable  
  - After elimination, system becomes **upper triangular**  
  - Back substitution solves the system from bottom up  

---

### Key points
1. Pivot = leading nonzero coefficient in current row  
2. Multiplier = (entry to eliminate) / (pivot)  
3. Elimination transforms system without changing its solution  
4. Upper triangular form allows systematic back substitution  
5. If pivot = 0, swap rows to continue elimination  
6. Process scales to any $n \times n$ system  

- **Magyarul**: a pivot és a multiplier a kiküszöbölés kulcsa, a háromszög rendszerből visszahelyettesítéssel oldjuk meg a változókat, a megoldás mindig ugyanaz marad.
## Breakdown of Elimination (detailed explanation)

Elimination usually produces a triangular system with **n pivots**, which leads directly to a solution.  
However, there are **three types of possible failures**:

---

#### 1. Permanent failure – no solution
- System example:
$$
\begin{cases}
x - 2y = 1 \\
3x - 6y = 11
\end{cases}
$$  
- Step: eliminate $x$ from the second equation  
  - Multiplier: $m = 3/1 = 3$  
  - Subtract $3 \cdot$ eq1 from eq2:  
$$
(3x - 6y) - 3(x - 2y) = 0x + 0y
$$  
- Right-hand side: $11 - 3\cdot1 = 8$  
- Resulting equation: $0 = 8$ → impossible, **no solution**  
- **Row picture**: two parallel lines, no intersection  
- **Column picture**: columns are multiples of each other, cannot combine to form $b$ in a different direction  
- **Explanation**: elimination detects inconsistency naturally when a zero pivot would have to divide the nonzero right-hand side.  
![[Pasted image 20251001191135.png]]
---

#### 2. Failure – infinitely many solutions
- Change $b = (1,3)$:  
$$
\begin{cases}
x - 2y = 1 \\
3x - 6y = 3
\end{cases}
$$  
- Elimination: subtract $3 \cdot$ eq1 from eq2 → $0y = 0$  
- Result: **one pivot only**, $y$ is "free"  
- Solution: $x = 1 + 2y$, $y$ arbitrary  
- **Row picture**: two lines coincide → infinitely many points of intersection  
- **Column picture**: $b$ lies on the span of the first column → infinitely many combinations possible  
- **Explanation**: singular systems can have infinitely many solutions, elimination reveals the free variable when pivot is missing.  

---

#### 3. Temporary failure – pivot = 0
- Example:  
$$
\begin{cases}
0x + 2y = 4 \\
3x - 2y = 5
\end{cases}
$$  
- First pivot = 0 → cannot divide  
- **Solution**: exchange rows  
$$
\begin{cases}
3x - 2y = 5 \\
2y = 4
\end{cases}
$$  
- Now pivots are nonzero → elimination works  
- Back substitution: $y=2$, $x=3$  
- **Row and column pictures**: normal, solution exists  
- **Explanation**: row swaps allow continuation if pivot is zero  

---

### Gaussian Elimination – 3×3 Example

System:  
$$
\begin{cases}
2x + 4y - 2z = 2 \\
4x + 9y - 3z = 8 \\
-2x - 3y + 7z = 10
\end{cases}
$$  

**Step 1: eliminate x from eq2 and eq3**  
- Pivot: $a_{11} = 2$  
- Multiplier for eq2: $m_{21} = 4/2 = 2$  
- Subtract $2 \cdot$ eq1 from eq2:  
$$
(4x + 9y - 3z) - 2(2x + 4y - 2z) = y + z
$$  
- Subtract eq1 from eq3: multiplier $m_{31} = -2/2 = -1$ → eq3 becomes $y + 5z$  

**Step 2: eliminate y from eq3**  
- Pivot: eq2, coefficient of $y = 1$  
- Multiplier: $m = 1/1 = 1$  
- Subtract eq2 from eq3 → $4z = 8$ → $z=2$  

**Step 3: back substitution**  
- eq2: $y + z = 4 \Rightarrow y + 2 = 4 \Rightarrow y = 2$  
- eq1: $2x + 4y - 2z = 2 \Rightarrow 2x + 8 - 4 = 2 \Rightarrow 2x = -2 \Rightarrow x=-1$  

- **Solution**: $(x, y, z) = (-1, 2, 2)$  

- **Row picture**: three planes intersect at one point  
- **Column picture**: linear combination of columns gives $b$ using coefficients $(-1,2,2)$  
![[Pasted image 20251001191201.png]]
---

### Elimination from A to U – Detailed Explanation

Gaussian elimination for **n×n systems** follows the same pattern as smaller examples.  

---

#### Forward Elimination (A → U)

1. **Column 1**:  
   - Use the first pivot (top-left element) to eliminate all entries **below** it in the first column.  
   - Each row below is updated: subtract a multiple of the pivot row so that the first column becomes **0** below the pivot.  
   - Multiplier formula:  
   $$
   m_{ij} = \frac{a_{ij}}{pivot_i}, \quad j>i
   $$  
   - **Explanation**: multiplier scales the pivot row to cancel the target entry.  

2. **Column 2**:  
   - Move to the next pivot (second row, second column).  
   - Use this pivot to eliminate all entries below it in the second column.  
   - Repeat the same multiplier procedure.  

3. **Columns 3 to n**:  
   - Continue pivoting down the diagonal.  
   - Each pivot must be **nonzero**; if zero, swap rows.  
   - After the final column, the matrix is **upper triangular U**.  

- **Result**: forward elimination converts $Ax = b$ into $Ux = c$.  
- **Nonsingular system**: full set of n nonzero pivots → exactly one solution.  
- **Singular system**: missing pivots → no solution or infinitely many solutions.  

---

#### Example – 3×3 System

Original system:  
$$
\begin{cases}
x + y + z = 6 \\
x + 2y + 2z = 9 \\
x + 2y + 3z = 10
\end{cases}
$$  

**Step 1: Forward elimination**  
- Eliminate $x$ from eq2 and eq3 using eq1 (pivot = 1)  
- eq2 new: $(x + 2y + 2z) - 1*(x + y + z) = y + z = 3$  
- eq3 new: $(x + 2y + 3z) - 1*(x + y + z) = y + 2z = 4$  

**Step 2: Eliminate $y$ from eq3**  
- Pivot = eq2, coefficient of $y = 1$  
- eq3 new: $(y + 2z) - 1*(y + z) = z = 1$  

**Step 3: Back substitution**  
- eq3 → $z=1$  
- eq2 → $y + z = 3 \Rightarrow y = 2$  
- eq1 → $x + y + z = 6 \Rightarrow x = 3$  

- **Solution**: $(x, y, z) = (3, 2, 1)$  

---

#### Row and Column Perspective

- **Row picture**: three planes intersect at one point, which is the solution.  
- **Column picture**: the columns of $A$ combine using the solution coefficients $(3,2,1)$ to give $b = (6, 9, 10)$.  
- **Triangle representation**: after elimination, $Ux = c$ forms an upper triangular system:  
$$
Ux = c = 
\begin{cases}
x + y + z = 6 \\
y + z = 3 \\
z = 1
\end{cases}
$$  

**Explanation of multipliers**:  
- Each step uses the pivot to scale and cancel variables in rows below.  
- The diagonal elements of U (the pivots) are revealed progressively.  
- Forward elimination ensures the system is ready for **back substitution**, solving from the bottom row upwards.  

- **Magyarul**: az elimináció során a diagonális elemek (pivotok) a változók sorrendjét adják, multiplikátorokkal nullázzuk ki az alatta lévő elemeket, majd visszaszámolással kapjuk meg a megoldást. A sorok geometriailag síkokat, az oszlopok lineáris kombinációkat képviselnek.